Quotify/BinRel.lean
@@ -63,15 +63,23 @@ def getArgType (rel : Expr) (numParams : Nat) : MetaM GetArgTypeResult := do
       let failedRelType ← mkLambdaFVars fvars relType
       return .illformedType failedRelType
 
+public structure LevelParamNormalization where
+  original : List Name
+  normal   : List Name
+
+instance : EmptyCollection LevelParamNormalization where
+  emptyCollection := { original := [], normal := [] }
+
 /--
 Normalizes the names of level parameters in `expr`. We rename them to `_uvar.0`, `_uvar.1`, etc.
 -/
-def normalizeLevelParams (expr : Expr) : MetaM (Expr × List Name) := do
+def normalizeLevelParams (expr : Expr) : MetaM (Expr × LevelParamNormalization) := do
   let { params, .. } := collectLevelParams {} expr
   let normNames := params.mapIdx fun idx _ => Name.num `_uvar idx
   let normParams := normNames.map mkLevelParam
   let expr := expr.instantiateLevelParamsArray params normParams
-  return (expr, normNames.toList)
+  let norm := { original := params.toList, normal := normNames.toList }
+  return (expr, norm)
 
 -- **TODO** What sort of reduction does `reduce` actually perform?
 def reduceRelation (rel : Expr) : MetaM Expr := do
@@ -79,7 +87,7 @@ def reduceRelation (rel : Expr) : MetaM Expr := do
   return rel.eta
 
 public inductive FromExprResult where
-  | success (rel : BinRel)
+  | success (rel : BinRel) (levelParamNorm : LevelParamNormalization)
   | illformedType (type : Expr)
 
 /--
@@ -89,7 +97,7 @@ an expression of the form `λ m₁ … mₙ, rel m₁ … mₙ`, where `m₁ …
 `rel m₁ … mₙ` can itself be a `λ`, we keep track of how many arguments in the telescope parameterize
 the relation in `BinRel.numParams`. That
 -/
-def fromExpr (rel : Expr) : MetaM FromExprResult := do
+def fromExpr (rel : Expr) (normalizeLevels : Bool) : MetaM FromExprResult := do
   let rel ← instantiateMVars rel
   let rel ← reduceRelation rel
   -- Abstracts the relation over its parameters, which are (expected to be) represented as mvars. So
@@ -97,29 +105,33 @@ def fromExpr (rel : Expr) : MetaM FromExprResult := do
   let { expr := rel, mvars := relMVars, .. } ← abstractMVars rel
   -- The number of arguments parameterizing the binary relation.
   let numParams := relMVars.size
-  -- This step ensures that the names of universe parameters in `rel` are consistent (note that
+  -- This step ensures that the names of level parameters in `rel` are consistent (note that
   -- `abstractMVars` above ensured that there are no level mvars). If we did not do this, then
-  -- "obviously" equal `BinRel`s would not compare as equal due to mismatching universe parameter
-  -- names.
-  let (rel, levelParams) ← normalizeLevelParams rel
+  -- "obviously" equal `BinRel`s would not compare as equal due to different level parameter names.
+  let (rel, levelParamNorm) ← if normalizeLevels then normalizeLevelParams rel else pure (rel, ∅)
   -- Gets the argument type, while also checking that `rel` is a homogeneous binary relation.
   match ← getArgType rel numParams with
-  | .success argType    => return .success { expr := rel, argType, numParams, levelParams }
-  | .illformedType type => return .illformedType type
+  | .illformedType type =>
+    return .illformedType type
+  | .success argType =>
+    let levelParams := levelParamNorm.normal
+    return .success { expr := rel, argType, numParams, levelParams } levelParamNorm
 
 public inductive FromFullyAppliedResult where
-  | success (rel : BinRel)
+  | success (rel : BinRel) (levelParamNorm : LevelParamNormalization)
   | illformedType (type : Expr)
   | missingArgs (numArgs : Nat)
 
 instance : Coe FromExprResult FromFullyAppliedResult where
   coe
-    | .success rel        => .success rel
-    | .illformedType type => .illformedType type
+    | .success rel levelParamNorm => .success rel levelParamNorm
+    | .illformedType type         => .illformedType type
 
 /--
 Given an `expr` which reduces to the form `r a₁ … aₙ lhs rhs`, where `r a₁ … aₙ : α → α → Prop`,
 returns a `BinRel` for `r a₁ … aₙ`. See `BinRel.fromExpr` for more information.
+
+Note, when `normalizeLevels = true` the types of `lhs` and `rhs` will still not be level-normalized.
 
 ---
 
@@ -135,7 +147,7 @@ distinction between the binary relation and its arguments. For example, consider
 `∀ x, x ∈ a ↔ x ∈ b`, which is not an application containing the elements being compared, so it is
 not immedaitely obvious what the binary relation should be.
 -/
-public def fromFullyApplied (app : Expr) : MetaM FromFullyAppliedResult := do
+public def fromFullyApplied (app : Expr) (normalizeLevels := true) : MetaM FromFullyAppliedResult := do
   -- We used to run `let app ← withConfig ({ · with beta := false }) do whnf app` at the start. This
   -- was supposed to unfold the head such that any potential arguments "hidden" in the head become
   -- visible. For example, given a definition `Empty {α} (l : List α) : Prop := l = []`, this
@@ -150,7 +162,7 @@ public def fromFullyApplied (app : Expr) : MetaM FromFullyAppliedResult := do
   let numArgs := app.getAppNumArgs'
   unless app.getAppNumArgs' ≥ 2 do return .missingArgs numArgs
   let rel := app.stripArgsN 2
-  fromExpr rel
+  fromExpr rel normalizeLevels
 
 public def fromTerm (rel : Term) : TermElabM BinRel := do
   let relExpr ← elabTerm rel none
@@ -160,7 +172,7 @@ public def fromTerm (rel : Term) : TermElabM BinRel := do
   let relExpr ← etaExpand relExpr
   let (_, _, fullyAppliedRelExpr) ← lambdaMetaTelescope relExpr
   match ← BinRel.fromFullyApplied fullyAppliedRelExpr with
-  | .success binRel => return binRel
+  | .success binRel _ => return binRel
   | .missingArgs numArgs =>
     throwError "The type of {indentExpr fullyAppliedRelExpr}\nis not compatible with `quotify`. It \
                 is expected to be a binary relation, but takes {numArgs} arguments."
@@ -184,15 +196,22 @@ returns `(params : Array Expr) × (lmvars : List Level) × (rel : Expr) × (argT
 `params` being the mvars for `a₁ … aₙ`, `lmvars` being the the level mvars instantiated for
 `binRel.levelParams`, and `rel` and `argType` begin instantiated to `r params` and `argType params`
 and the level mvars respectively.
+
+If `levels := false`, level parameters will not be instantiated with level mvars.
 -/
-public def metaTelescope (binRel : BinRel) : MetaM (Array Expr × List Level × Expr × Expr) := do
+public def metaTelescope (binRel : BinRel) (levels := true) :
+    MetaM (Array Expr × List Level × Expr × Expr) := do
+  let mut expr := binRel.expr
+  let mut argType := binRel.argType
+  let mut freshLMVars := []
   -- It's important that we instantiate the level params with level mvars *before* we telescope, as
   -- otherwise the types of the created (expr) mvars still refer to the level params.
-  let freshLMVars       ← mkFreshLevelMVars binRel.levelParams.length
-  let expr             := binRel.expr.instantiateLevelParams binRel.levelParams freshLMVars
-  let argType          := binRel.argType.instantiateLevelParams binRel.levelParams freshLMVars
-  let (params, _, rel)  ← lambdaMetaTelescope expr (maxMVars? := binRel.numParams)
-  let argType           ← instantiateLambda argType params
+  if levels then
+    freshLMVars ← mkFreshLevelMVars binRel.levelParams.length
+    expr       := binRel.expr.instantiateLevelParams binRel.levelParams freshLMVars
+    argType    := binRel.argType.instantiateLevelParams binRel.levelParams freshLMVars
+  let (params, _, rel) ← lambdaMetaTelescope expr (maxMVars? := binRel.numParams)
+  argType              ← instantiateLambda argType params
   return (params, freshLMVars, rel, argType)
 
 public def synthSetoid? (binRel : BinRel) : MetaM (Option Expr) := do
@@ -205,48 +224,28 @@ public def synthSetoid? (binRel : BinRel) : MetaM (Option Expr) := do
 public def forThm? (thmInfo : TheoremVal) : MetaM (Option BinRel) := do
   let thmType := thmInfo.type
   let (_, _, fullyAppliedThmType) ← forallMetaTelescopeReducing thmType
-  let .success binRel ← BinRel.fromFullyApplied fullyAppliedThmType | return none
+  let .success binRel _ ← BinRel.fromFullyApplied fullyAppliedThmType | return none
   return binRel
 
+theorem iff_quotient_eq (rel : α → α → Prop) (equiv : Equivalence rel) :
+    ∀ lhs rhs, rel lhs rhs ↔ (Quotient.mk ⟨rel, equiv⟩ lhs = .mk ⟨rel, equiv⟩ rhs) :=
+  fun _ _ => ⟨(Quotient.sound ·), (Quotient.exact ·)⟩
+
 /--
-Given a `BinRel` of the form `λ a₁ … aₙ, r a₁ … aₙ`, and a proof that it is an equivalence, returns
-the corresponding relation over quotients
-`λ a₁ … aₙ lhs rhs, Quotient.mk (r a₁ … aₙ) lhs = Quotient.mk (r a₁ … aₙ) rhs`, where the setoid
-instance is constructed on-the-fly.
-
----
-
-Note: We expect `binRel` and `equiv` to be abstracted over the same parameters.
+Returns a proof of `BinRel.iff_quotient_eq` instantiated for the given `BinRel` and equivalence
+proof. If the relation is not fully applied, the proof remains abstracted over the remaining
+parameters. That is, it has type `∀ a₁ … aₙ, ∀ lhs rhs, binRel lhs rhs ↔ ⟦lhs⟧ = ⟦rhs⟧`.
 -/
-public def toQuotient (binRel : BinRel) (equiv : Expr) : MetaM Expr := do
+public def mkIffQuotientEq (binRel : BinRel) (equiv : Expr) : MetaM Expr := do
   binRel.telescope fun params rel argType => do
-    withLocalDecl `lhs .default argType fun lhs => do
-      withLocalDecl `rhs .default argType fun rhs => do
-        let equiv   ← instantiateLambda equiv params
-        let level   ← getLevel argType
-        let setoid := mkApp3 (.const ``Setoid.mk [level]) argType rel equiv
-        let eqLhs  := mkApp3 (.const ``Quotient.mk [level]) argType setoid lhs
-        let eqRhs  := mkApp3 (.const ``Quotient.mk [level]) argType setoid rhs
-        let eq      ← mkEq eqLhs eqRhs
-        let vars   := params ++ #[lhs, rhs]
-        mkLambdaFVars vars eq
-
-theorem eq_toQuotient (binRel : α → α → Prop) (equiv : Equivalence binRel) :
-    binRel = (Quotient.mk ⟨binRel, equiv⟩ · = .mk ⟨binRel, equiv⟩ ·) :=
-  funext fun _ => funext fun _ => propext ⟨(Quotient.sound ·), (Quotient.exact ·)⟩
+    let equiv  ← instantiateLambda equiv params
+    let level  ← getLevel argType
+    let proof := mkApp3 (.const ``Quotify.BinRel.iff_quotient_eq [level]) argType rel equiv
+    mkLambdaFVars params proof
 
 public structure Match where
   params : Array Expr
   levels : List Level
-
--- **TODO** What about level parameters?
-public def Match.instantiate (mat : Match) (e : Expr) : MetaM Expr := do
-  let e ← instantiateLambda e mat.params
-  -- If `m` was obtained by matching a target which is not fully applied, then `params` will contain
-  -- mvars for those arguments which are to remain abstracted. Thus, after instantiating `m.params`,
-  -- we abstract these mvars again.
-  let mvarParams := mat.params.filter (·.isMVar)
-  mkLambdaFVars mvarParams e
 
 /--
 Tries to match a given `target` against a `pattern` up to definitional equality. If the match
@@ -257,10 +256,13 @@ Matching is asymmetric in that the `pattern` must be more abstract than the `tar
 way around.
 
 If `target` is not fully applied, i.e. it contains abstracted parameters, then the resulting `Match`
-will contain mvars for these parameters.
+will contain mvars for these parameters. In contrast, level parameters will not be replaced by level
+mvars.
 -/
 public def match? (pattern target : BinRel) : MetaM (Option Match) := do
-  let (_, _, target, _) ← target.metaTelescope
+  -- We do not want to instantiate the `target`'s level parameters with level mvars, as the its
+  -- level parameters are sufficient to "travel" between contexts.
+  let (_, _, target, _) ← target.metaTelescope (levels := false)
   -- We bump the mvar context depth so that only `pattern`s (abstracted) parameters can be matched
   -- but not the other way around. For example, this means that `@List.Param ?α` can be matched
   -- against `@List.Param Nat`, but not vice versa.
