Quotify/Tactic.lean
@@ -1,0 +1,38 @@
+module
+public meta import Lean.Elab.Tactic
+public meta import Lean.Meta.Tactic.Simp
+public meta import Quotify.Attribute
+public meta import Quotify.Lean
+
+open Lean Meta Elab Tactic
+
+namespace Quotify
+
+-- **BUG** If we run in a reverted context, then `binRel` may contain fvars from the outer context.
+
+/--
+Replaces all occurrences of `binRel` in the goal and local context with the corresponding quotient
+equality relation, proven equal by `iffQuotEq`.
+-/
+meta def swapRelation (binRel : BinRel) (iffQuotEq : Expr) : TacticM Unit :=
+  -- We use `simp only` instead of `rw`, so that *all* occurrences are rewritten.
+  inRevertedCtx do
+    let goal             ← getMainGoal
+    let iffQuotEqSimpThm ← SimpTheorems.add {} (.other `Quotify.swapRelation) binRel.levelParams.toArray iffQuotEq
+    let simpCtx          ← Simp.mkContext (simpTheorems := #[iffQuotEqSimpThm])
+    -- **TODO** Is this always type correct? Or can we run into "motive not type correct" issues?
+    let (some (_, goal), _) ← simpGoal goal simpCtx
+      | throwError "`quotify` failed to swap the relation {indentExpr binRel.expr}\nfor equality \
+                    of quotients."
+    replaceMainGoal [goal]
+
+elab tk:"quotify" : tactic =>
+  withRef tk <| withMainContext do
+    let goalType ← getMainTarget
+    let .success binRel _ ← BinRel.fromFullyApplied goalType (normalizeLevels := false)
+      | throwError "`quotify` failed to find a binary relation in the goal."
+    let some setoid ← extension.getMatchingSetoid? binRel
+      | throwError "`quotify` failed to find a `{.ofConstName ``Setoid}` marked with `[quotify]` \
+                     for the relation {indentExpr binRel.expr}"
+    let iffQuotEq ← binRel.mkIffQuotientEq setoid.equiv.proof
+    swapRelation binRel iffQuotEq
