Quotify/Unexpanders.lean
@@ -1,5 +1,10 @@
 import Quotify.Mathlib
 
+@[app_unexpander Quotient.mk]
+def unexpandMk : Lean.PrettyPrinter.Unexpander
+  | `($_ $_ $t:term) => `(⟦$t⟧)
+  | _ => throw ()
+
 @[app_unexpander Quotient.lift]
 def unexpandLift : Lean.PrettyPrinter.Unexpander
   | `($_ $t:term ⋯) => `(⟦$t⟧)
