Tests/Quot.lean
@@ -3,48 +3,22 @@ import Quotify.Command
 attribute [quotify] List.isSetoid
 
 /--
-info: fun x_0 lhs rhs => Quotient.mk { r := List.Perm, iseqv := ⋯ } lhs = Quotient.mk { r := List.Perm, iseqv := ⋯ } rhs
+info: ∀ (x_0 : Type _uvar.0) (lhs rhs : List x_0),
+  lhs.Perm rhs ↔ Quotient.mk { r := List.Perm, iseqv := ⋯ } lhs = Quotient.mk { r := List.Perm, iseqv := ⋯ } rhs
 -/
 #guard_msgs in
 #quotify_quot List.Perm
 
 /--
-info: fun α lhs rhs => Quotient.mk { r := List.Perm, iseqv := ⋯ } lhs = Quotient.mk { r := List.Perm, iseqv := ⋯ } rhs
+info: ∀ (α : Type _uvar.0) (lhs rhs : List α),
+  lhs.Perm rhs ↔ Quotient.mk { r := List.Perm, iseqv := ⋯ } lhs = Quotient.mk { r := List.Perm, iseqv := ⋯ } rhs
 -/
 #guard_msgs in
 #quotify_quot ((· ≈ ·) : List ?α → List ?α → Prop)
 
 /--
-info: fun lhs rhs => Quotient.mk { r := List.Perm, iseqv := ⋯ } lhs = Quotient.mk { r := List.Perm, iseqv := ⋯ } rhs
+info: ∀ (lhs rhs : List Nat),
+  lhs.Perm rhs ↔ Quotient.mk { r := List.Perm, iseqv := ⋯ } lhs = Quotient.mk { r := List.Perm, iseqv := ⋯ } rhs
 -/
 #guard_msgs in
 #quotify_quot @List.Perm Nat
-
-/- **TODO** Look into the level parameter name mismatch of the `BinRel` and the equivalence proof.
-
-fun (x_0 : Type _uvar.0) (lhs rhs : List.{_uvar.0} x_0) =>
-  @Eq.{_uvar.0 + 1}
-    (@Quotient.{_uvar.0 + 1} (List.{_uvar.0} x_0)
-      (@Setoid.mk.{_uvar.0 + 1} (List.{_uvar.0} x_0) (@List.Perm.{_uvar.0} x_0)
-        (@Setoid.iseqv.{u_1 + 1} (List.{u_1} x_0)
-          ((fun (α : Type u_1) =>
-              (fun (α : Type u_1) => @Setoid.mk.{u_1 + 1} (List.{u_1} α) (@List.Perm.{u_1} α) (List.Perm.eqv.{u_1} α))
-                α)
-            x_0))))
-    (@Quotient.mk.{_uvar.0 + 1} (List.{_uvar.0} x_0)
-      (@Setoid.mk.{_uvar.0 + 1} (List.{_uvar.0} x_0) (@List.Perm.{_uvar.0} x_0)
-        (@Setoid.iseqv.{u_1 + 1} (List.{u_1} x_0)
-          ((fun (α : Type u_1) =>
-              (fun (α : Type u_1) => @Setoid.mk.{u_1 + 1} (List.{u_1} α) (@List.Perm.{u_1} α) (List.Perm.eqv.{u_1} α))
-                α)
-            x_0)))
-      lhs)
-    (@Quotient.mk.{_uvar.0 + 1} (List.{_uvar.0} x_0)
-      (@Setoid.mk.{_uvar.0 + 1} (List.{_uvar.0} x_0) (@List.Perm.{_uvar.0} x_0)
-        (@Setoid.iseqv.{u_1 + 1} (List.{u_1} x_0)
-          ((fun (α : Type u_1) =>
-              (fun (α : Type u_1) => @Setoid.mk.{u_1 + 1} (List.{u_1} α) (@List.Perm.{u_1} α) (List.Perm.eqv.{u_1} α))
-                α)
-            x_0)))
-      rhs)
--/
