Tests/SwapRelation.lean
@@ -1,0 +1,22 @@
+import Quotify.Tactic
+import Quotify.Unexpanders
+
+attribute [quotify] List.isSetoid
+
+/--
+error: unsolved goals
+l₁ l₂ : List Nat
+h : ⟦l₁.reverse⟧ = ⟦l₂.reverse⟧
+⊢ ⟦l₁⟧ = ⟦l₂⟧
+-/
+#guard_msgs in
+example (l₁ l₂ : List Nat) (h : l₁.reverse.Perm l₂.reverse) : l₁.Perm l₂ := by
+  quotify
+
+-- **BUG** Running in a reverted context produces dangling fvars.
+set_option pp.explicit true in
+example (l₁ l₂ : List α) (h : l₁.reverse.Perm l₂.reverse) : l₁.Perm l₂ := by
+  quotify
+
+example (l₁ l₂ : List Nat) : l₁ ≈ l₂ := by
+  quotify
